\input{lib}

\begin{document}

\begin{align*}
    &\begin{array}{ll}
        t_{0}t_{5} = t_{1}t_{3} - t_{3}t_{3} + t_{3}t_{6}&
        t_{0}t_{6} = t_{3}t_{3} - t_{3}t_{4}\\
        t_{0}t_{7} = t_{3}t_{4} - t_{4}t_{4}&
        t_{0}t_{8} = t_{3}t_{6} - t_{4}t_{6}\\
        t_{1}t_{4} = t_{3}t_{3} - t_{3}t_{6}&
        t_{1}t_{7} = t_{3}t_{6} - t_{6}t_{6}\\
        t_{1}t_{8} = t_{5}t_{6}&
        t_{2}t_{4} = t_{0}t_{3} - t_{3}t_{3} + t_{3}t_{4}\\
        t_{2}t_{5} = t_{1}t_{1} - t_{1}t_{3} + t_{3}t_{5}&
        t_{2}t_{6} = t_{1}t_{3} - t_{3}t_{3} + t_{3}t_{6}\\
        t_{2}t_{7} = t_{3}t_{3} - t_{3}t_{6} - t_{3}t_{4} + t_{4}t_{6}&
        t_{2}t_{8} = t_{3}t_{5} - t_{3}t_{6} + t_{6}t_{6}\\
        t_{3}t_{8} = t_{6}t_{6}&
        t_{4}t_{5} = t_{3}t_{6} - t_{6}t_{6}\\
        t_{4}t_{8} = t_{6}t_{7}&
        t_{5}t_{7} = t_{6}t_{6} - t_{6}t_{8}
    \end{array}\\
    &\left[\begin{array}{cccccc}
        t_0 & t_2 & t_0   &   t_3 - t_4       &  \\
        t_6 & t_5 & t_1   &   t_5
    \end{array}\right]
    \left[\begin{array}{cc}
        t_1 & t_0 \\
        t_5 & t_3-t_4
    \end{array}\right]
\end{align*}
\begin{align*}
    \begin{array}{ll}
        t_{0}t_{5} = t_{1}t_{3} - t_{3}t_{3} + t_{3}t_{6}&
        t_{0}t_{6} = t_{3}t_{3} - t_{3}t_{4}\\
        t_{0}t_{7} = t_{3}t_{4} - t_{4}t_{4}&
        t_{0}t_{8} = t_{3}t_{6} - t_{4}t_{6}\\
        t_{1}t_{4} = t_{3}t_{3} - t_{3}t_{6}&
        t_{1}t_{7} = t_{3}t_{6} - t_{6}t_{6}\\
        t_{1}t_{8} = t_{5}t_{6}&
        t_{2}t_{4} = t_{0}t_{3} - t_{3}t_{3} + t_{3}t_{4}\\
        t_{2}t_{5} = t_{1}t_{1} - t_{1}t_{3} + t_{3}t_{5}&
        t_{2}t_{6} = t_{0}t_{5}\\
        t_{2}t_{7} = t_{0}t_{6} - t_{0}t_{8}&
        t_{2}t_{8} = t_{3}t_{5} - t_{3}t_{6} + t_{6}t_{6}\\
        t_{3}t_{8} = t_{6}t_{6}&
        t_{4}t_{5} = t_{0}t_{8}\\
        t_{4}t_{8} = t_{6}t_{7}&
        t_{5}t_{7} = t_{6}t_{6} - t_{6}t_{8}
    \end{array}
\end{align*}
\begin{align*}
    \begin{array}{ll}
        t_{0}t_{5} = t_{1}(t_{3} - t_{4}) = t_{2}t_{6}&
        t_{0}t_{6} = t_{3}(t_{3} - t_{4})\\
        t_{0}t_{7} = t_{4}(t_{3} - t_{4})&
        t_{0}t_{8} = t_{6}(t_{3} - t_{4})\\
        t_{1}t_{4} = t_{3}(t_{3} - t_{6})&
        t_{1}t_{7} = t_{6}(t_{3} - t_{6}) = t_{4}t_{5} \\
        t_{1}t_{8} = t_{5}t_{6}&
        t_{2}t_{4} = t_{0}(t_{3} - t_{6})\\
        t_{2}t_{5} = t_{1}t_{1} - t_{1}t_{3} + t_{3}t_{5}&
        t_{2}t_{6} = t_{0}t_{5}\\
        t_{2}t_{7} = t_{0}(t_{6} - t_{8})&
        t_{2}t_{8} = t_{5}(t_{3} - t_{4})\\
        t_{3}t_{8} = t_{6}t_{6}&
        t_{4}t_{5} = t_{1}t_{7} \\
        t_{4}t_{8} = t_{6}t_{7}&
        t_{5}t_{7} = t_{6}(t_{6} - t_{8})
    \end{array}
\end{align*}
\begin{align*}
    \begin{array}{ll}
        t_{0}t_{5} = t_{1}t_{3} - t_{3}t_{3} + t_{3}t_{6}&
        t_{0}t_{6} = t_{3}(t_{3} - t_{4}) = t_{3}t_{3} - t_{3}t_{4}\\
        t_{0}t_{7} = t_{4}(t_{3} - t_{4}) = t_{3}t_{4} - t_{4}t_{4}&
        t_{0}t_{8} = t_{6}(t_{3} - t_{4}) = t_{3}t_{6} - t_{4}t_{6}\\
        t_{1}t_{4} = t_{3}(t_{3} - t_{6}) = t_{3}t_{3} - t_{3}t_{6}&
        t_{1}t_{7} = t_{6}(t_{3} - t_{6}) = t_{3}t_{6} - t_{6}t_{6}\\
        t_{1}t_{8} = t_{5}t_{6}&
        t_{2}t_{4} = t_{0}t_{3} - t_{3}t_{3} + t_{3}t_{4}\\
        t_{2}t_{5} = t_{1}t_{1} - t_{1}t_{3} + t_{3}t_{5}&
        t_{2}t_{6} = t_{1}t_{3} - t_{3}t_{3} + t_{3}t_{6}\\
        t_{2}t_{7} = t_{3}t_{3} - t_{3}t_{6} - t_{3}t_{4} + t_{4}t_{6}&
        t_{2}t_{8} = t_{3}t_{5} - t_{3}t_{6} + t_{6}t_{6}\\
        t_{3}t_{8} = t_{6}t_{6}&
        t_{4}t_{5} = t_{6}(t_{3} - t_{6}) = t_{3}t_{6} - t_{6}t_{6}\\
        t_{4}t_{8} = t_{6}t_{7}&
        t_{5}t_{7} = t_{6}(t_{6} - t_{8})
    \end{array}
\end{align*}
\begin{align*}
    t_{0}t_{5} 
    = t_{3}(t_{1} - (t_{3} - t_{6})) 
    = t_{1}t_{3} - t_{3}t_{3} + t_{3}t_{6}
\end{align*}
\begin{align*}
    t_{0}t_{6}
    = t_{3}(t_{3} - t_{4})
    = t_{3}t_{3} - t_{3}t_{4}
\end{align*}
\begin{align*}
    t_{0}t_{7}
    = t_{4}(t_{3} - t_{4})
    = t_{3}t_{4} - t_{4}t_{4}
\end{align*}
\begin{align*}
    t_{0}t_{8}
    = t_{6}(t_{3} - t_{4})
    = t_{3}t_{6} - t_{4}t_{6}
\end{align*}
\begin{align*}
    t_{1}t_{4}
    = t_{3}(t_{3} - t_{6})
    = t_{3}t_{3} - t_{3}t_{6}
\end{align*}
\begin{align*}
    t_{1}t_{7} 
    = t_{6}(t_{3} - t_{6})
    = t_{3}t_{6} - t_{6}t_{6}
\end{align*}
\begin{align*}
    t_{1}t_{8} = t_{5}t_{6}
\end{align*}
\begin{align*}
    t_{2}t_{4} 
    = t_{0}t_{3} - t_{3}t_{3} + t_{3}t_{4}
    = t_{0}t_{3} - t_{3}t_{3} + t_{3}t_{4}
\end{align*}
\begin{align*}
    t_{2}t_{5}
    = t_{1}t_{1} - t_{1}t_{3} + t_{3}t_{5}
    = t_{1}t_{1} - t_{1}t_{3} + t_{3}t_{5}
\end{align*}
\begin{align*}
    t_{2}t_{6} 
    = t_{1}t_{3} - t_{3}t_{3} + t_{3}t_{6}
    = t_{1}t_{3} - t_{3}t_{3} + t_{3}t_{6}
\end{align*}
\begin{align*}
    t_{2}t_{7} 
    = (t_{3} - t_{6})(t_{3} - t_{4})
    = t_{3}(t_{3} - t_{6}) - t_{4}(t_{3} - t_{6})
    = t_{3}t_{3} - t_{3}t_{6} - t_{3}t_{4} + t_{4}t_{6}
\end{align*}
\begin{align*}
    t_{2}t_{8} 
    = t_{3}t_{5} - t_{3}t_{6} + t_{6}t_{6}
    = t_{3}t_{5} - t_{3}t_{6} + t_{6}t_{6}
\end{align*}
\begin{align*}
    t_{3}t_{8} = t_{6}t_{6}
\end{align*}
\begin{align*}
    t_{4}t_{5} 
    = t_{6}(t_{3} - t_{6})
    = t_{3}t_{6} - t_{6}t_{6}
\end{align*}
\begin{align*}t_{4}t_{8} = t_{6}t_{7}
\end{align*}
\begin{align*}
    t_{5}t_{7} 
    = t_{6}(t_{6} - t_{8})
    = t_{6}t_{6} - t_{6}t_{8}
\end{align*}

\end{document}
